concurrency/hashtable/HashTableRefiment.s.dfy
@@ -5,10 +5,14 @@ module HashTableRefiment refines
     TicketStubStateMachine(MapIfc, HashTableStubSSM),
     AsyncStateMachine(MapIfc, MapSpec))
 {
+  import opened KeyValueType
+  import MapSpec
+  import MapIfc
+
   import SSM = HashTableStubSSM
   import SM = StateMachine(MapIfc)
-  import CircularTable
-  import MapSpec
+  import opened CircularTable
+  import opened CircularRange
 
   // import A = TicketStubStateMachine(MapIfc, HashTableStubSSM)
   // import B = AsyncStateMachine(MapIfc, MapSpec)
@@ -42,8 +46,228 @@ module HashTableRefiment refines
   function I(s: A.Variables) : B.Variables
   {
     var m := CircularTable.I(s.table);
-    B.Variables(
-      MapSpec.Variables(m),
-      s.reqs, s.resps)
+    B.Variables(MapSpec.Variables(m), s.reqs, s.resps)
+  }
+
+  lemma InitRefinesInit(s: A.Variables)
+  {
+    CircularTable.EmptyTableEmptyMap(s.table);
+  }
+
+  lemma InsertRefinesMap(s: A.Variables, s': A.Variables, step: SSM.Step) 
+    returns (output: MapIfc.Output)
+    requires Inv(s) && Inv(s')
+    requires step.InsertStep? && SSM.NextStep(s, s', step)
+    requires step.input.InsertInput?
+    ensures MapSpec.Next(
+      MapSpec.Variables(I(s).s.m),
+      MapSpec.Variables(I(s').s.m),
+      MapIfc.Op(step.input, output))
+    ensures s'.reqs == s.reqs - {step.rid}
+    ensures s'.resps == s.resps[step.rid := output]
+  {
+    var InsertStep(rid, input, start, end) := step;
+    assert input.InsertInput?;
+    var InsertInput(key, value) := input;
+    var table, table' := s.table, s'.table;
+    var inserted := Full(key, value);
+
+    var p_range := Partial(hash(key), start);
+    ProbeRangeSufficient(table, key, p_range);
+    ContainmentEquivalent(table, key);
+    RightShiftPreservesMapping(table, table', inserted);
+
+    var si, si' := I(s), I(s');
+    var m, m' := si.s.m, si'.s.m;
+
+    assert m' == m[key := value];
+    output := MapIfc.InsertOutput(true);
+  }
+
+  lemma OverwriteRefinesMap(s: A.Variables, s': A.Variables, step: SSM.Step)
+    returns (output: MapIfc.Output)
+    requires Inv(s) && Inv(s')
+    requires step.OverwriteStep? && SSM.NextStep(s, s', step)
+    requires step.input.InsertInput?
+    ensures MapSpec.Next(
+      MapSpec.Variables(I(s).s.m),
+      MapSpec.Variables(I(s').s.m),
+      MapIfc.Op(step.input, output))
+    ensures s'.reqs == s.reqs - {step.rid}
+    ensures s'.resps == s.resps[step.rid := output]
+  {
+    var OverwriteStep(rid, input, end) := step;
+    assert input.InsertInput?;
+    var InsertInput(key, value) := input;
+    var table, table' := s.table, s'.table;
+    var inserted := Full(key, value);
+
+    ContainmentEquivalent(table, key);
+    OverwritePreservesMapping(table, table', end, inserted);
+
+    var si, si' := I(s), I(s');
+    var m, m' := si.s.m, si'.s.m;
+
+    assert m' == m[key := value];
+
+    output := MapIfc.InsertOutput(true);
+  }
+
+  lemma RemoveRefinesMap(s: A.Variables, s': A.Variables, step: SSM.Step)
+    returns (output: MapIfc.Output)
+    requires Inv(s) && Inv(s')
+    requires step.RemoveStep? && SSM.NextStep(s, s', step)
+    requires step.input.RemoveInput?
+    ensures MapSpec.Next(
+      MapSpec.Variables(I(s).s.m),
+      MapSpec.Variables(I(s').s.m),
+      MapIfc.Op(step.input, output))
+    ensures s'.reqs == s.reqs - {step.rid}
+    ensures s'.resps == s.resps[step.rid := output]
+  {
+    var RemoveStep(rid, input, start, end) := step;
+    var key := input.key;
+    var table, table' := s.table, s'.table;
+
+    ContainmentEquivalent(table, key);
+    LeftShiftPreservesMapping(table, table', key);
+
+    var si, si' := I(s), I(s');
+    var m, m' := si.s.m, si'.s.m;
+
+    assert m' == m - {key};
+    output := MapIfc.RemoveOutput(true);
+  }
+
+  lemma RemoveNotFoundRefinesMap(s: A.Variables, s': A.Variables, step: SSM.Step)
+    returns (output: MapIfc.Output)
+    requires Inv(s) && Inv(s')
+    requires step.RemoveNotFoundStep? && SSM.NextStep(s, s', step)
+    requires step.input.RemoveInput?
+    ensures MapSpec.Next(
+      MapSpec.Variables(I(s).s.m),
+      MapSpec.Variables(I(s').s.m),
+      MapIfc.Op(step.input, output))
+    ensures s'.reqs == s.reqs - {step.rid}
+    ensures s'.resps == s.resps[step.rid := output]
+  {
+    var RemoveNotFoundStep(rid, input, end) := step;
+    var key := input.key;
+    var table, table' := s.table, s'.table;
+    var p_range := Partial(hash(key), end);
+    ProbeRangeSufficient(table, key, p_range);
+
+    ContainmentEquivalent(table, key);
+
+    var si, si' := I(s), I(s');
+    var m, m' := si.s.m, si'.s.m;
+    assert key !in m;
+
+    output := MapIfc.RemoveOutput(false);
+  }
+
+  lemma QueryNotFoundRefinesMap(s: A.Variables, s': A.Variables, step: SSM.Step)
+    returns (output: MapIfc.Output)
+    requires Inv(s) && Inv(s')
+    requires step.QueryNotFoundStep? && SSM.NextStep(s, s', step)
+    requires step.input.QueryInput?
+    ensures MapSpec.Next(
+      MapSpec.Variables(I(s).s.m),
+      MapSpec.Variables(I(s').s.m),
+      MapIfc.Op(step.input, output))
+    ensures s'.reqs == s.reqs - {step.rid}
+    ensures s'.resps == s.resps[step.rid := output]
+  {
+    var QueryNotFoundStep(rid, input, end) := step;
+    var key := input.key;
+    var table, table' := s.table, s'.table;
+    var p_range := Partial(hash(key), end);
+    ProbeRangeSufficient(table, key, p_range);
+
+    ContainmentEquivalent(table, key);
+
+    var si, si' := I(s), I(s');
+    var m, m' := si.s.m, si'.s.m;
+    assert key !in m;
+
+    output := MapIfc.QueryOutput(QueryResult.NotFound);
+  }
+
+  lemma QueryFoundRefinesMap(s: A.Variables, s': A.Variables, step: SSM.Step)
+    returns (output: MapIfc.Output)
+    requires Inv(s) && Inv(s')
+    requires step.QueryFoundStep? && SSM.NextStep(s, s', step)
+    requires step.input.QueryInput?
+    ensures MapSpec.Next(
+      MapSpec.Variables(I(s).s.m),
+      MapSpec.Variables(I(s').s.m),
+      MapIfc.Op(step.input, output))
+    ensures s'.resps == s.resps[step.rid := output]
+  {
+    var QueryFoundStep(rid, input, end) := step;
+    var key := input.key;
+    var table := s.table;
+
+    ContainmentEquivalent(table, key);
+
+    var si, si' := I(s), I(s');
+    var m := si.s.m;
+
+    assert key in m && m[key] == table[end].value.value;
+    output := MapIfc.QueryOutput(QueryResult.Found(m[key]));
+  }
+
+  lemma InternalRefinesMap(s: A.Variables, s': A.Variables)
+    requires Inv(s)
+    requires SSM.Internal(s, s')
+    ensures Inv(s')
+    ensures B.Next(I(s), I(s'), ifc.InternalOp)
+  {
+    var step: SSM.Step :| SSM.NextStep(s, s', step); 
+    SSM.NextStepPreservesInv(s, s');
+
+    var si, si' := I(s), I(s');
+
+    var rid, input := step.rid, step.input;
+
+    var output;
+
+    if step.InsertStep? {
+      output := InsertRefinesMap(s, s', step);
+    } else if step.OverwriteStep? {
+      output := OverwriteRefinesMap(s, s', step);
+    } else if step.QueryFoundStep? {
+      output := QueryFoundRefinesMap(s, s', step);
+    } else if step.QueryNotFoundStep? {
+      output := QueryNotFoundRefinesMap(s, s', step);
+    } else if step.RemoveStep? {
+      output := RemoveRefinesMap(s, s', step);
+    } else if step.RemoveNotFoundStep? {
+      output := RemoveNotFoundRefinesMap(s, s', step);
+    } else {
+      assert false;
+    }
+
+    assert B.Next(si, si', ifc.InternalOp) by {
+      assert B.InteralNext(rid, input, output, si, si');
+    }
+  }
+
+  lemma NextRefinesNext(s: A.Variables, s': A.Variables, op: ifc.Op)
+  {
+    match op
+      case Start(rid, input) =>
+        assert s' == s.(reqs := s.reqs[rid := input]);
+        assert I(s') == I(s).(reqs := I(s).reqs[rid := input]);
+      case End(rid, output) =>
+        assert s == s'.(resps := s'.resps[rid := output]);
+        assert I(s) == I(s').(resps := I(s').resps[rid := output]);
+      case InternalOp => {
+        assert exists shard, shard', rest :: A.InternalNext(s, s', shard, shard', rest);
+        var shard, shard', rest :| A.InternalNext(s, s', shard, shard', rest);
+        SSM.InternalPreservesInv(shard, shard', rest);
+        SSM.InternalMonotonic(shard, shard', rest);
+        InternalRefinesMap(s, s');
+      }
   }
 }
